\documentclass[multi=math, crop, convert]{standalone}
\usepackage{physics}

\begin{document} 

\begin{math}
%\begin{equation*}
    \ket{\Psi} = \frac{1}{\sqrt{2}} \ket{0} + \frac{1}{\sqrt{2}} \ket{1}
%\end{equation*}
\end{math}

\begin{math}
OFF = \ket{0}
\end{math}

\begin{math}
ON = \ket{1}
\end{math}

\begin{math}
NOT\ket{0} = \ket{1}
\end{math}

\begin{math}
NOT\ket{1} = \ket{0}
\end{math}

\begin{math}
\hat{N}\ket{0} = \ket{1}
\end{math}

\begin{math}
	\hat{N}\ket{00}
\end{math}

\begin{math}
	\hat{A}\ket{0}
\end{math}

\begin{math}
\hat{N}\ket{1} = \ket{0}
\end{math}

\begin{math}
OFF, OFF = \ket{0} \otimes \ket{0}
\end{math}

\begin{math}
OFF, OFF = \ket{00}
\end{math}

\begin{math}
OFF, ON = \ket{0} \otimes \ket{1}
\end{math}

\begin{math}
OFF, ON = \ket{01}
\end{math}

\begin{math}
	\begin{matrix}
		\hat{N}\ket{0} = \ket{1}\\
		\hat{N}\ket{1} = \ket{0}
	\end{matrix}
\end{math}

\begin{math}
	\begin{matrix}
		\hat{A}\ket{00} = \ket{0}\\
		\hat{A}\ket{01} = \ket{0}\\
		\hat{A}\ket{10} = \ket{0}\\
		\hat{A}\ket{11} = \ket{1}
	\end{matrix}
\end{math}

\begin{math}
	\begin{matrix}
		\hat{O}\ket{00} = \ket{0}\\
		\hat{O}\ket{01} = \ket{1}\\
		\hat{O}\ket{10} = \ket{1}\\
		\hat{O}\ket{11} = \ket{1}
	\end{matrix}
\end{math}

\begin{math}
\hat{N}\hat{O}\ket{11} = \hat{N}\ket{1} = \ket{0}
\end{math}

\begin{math}
	\hat{N}\hat{N}\ket{0} = \hat{N}\ket{1} = \ket{0}
\end{math}

\begin{math}
\hat{A}\hat{O}\ket{11} = \hat{A}\ket{1} = 0
\end{math}

\begin{math}
\ket{0} = \begin{pmatrix}
	1 \\
	0
\end{pmatrix}
\end{math}

\begin{math}
\ket{1} = \begin{pmatrix}
	0 \\
	1
\end{pmatrix}
\end{math}

\begin{math}
	\ket{\Psi} = \alpha\ket{0} + \beta\ket{1} 
\end{math}

\begin{math}
	\abs{\alpha}^2 + \abs{\beta}^2 = 1
\end{math}

\begin{math}
	\hat{E}\ket{\Psi} = \hat{E}(\alpha\ket{0} + \beta\ket{1})
\end{math}

\begin{math}
	\hat{E}\ket{\Psi} = \hat{E}(\alpha\ket{0} + \beta\ket{1}) 
\end{math}

\begin{math}
	\ket{\Psi} = \alpha_0\ket{0} + \beta_0\ket{1} 
\end{math}

\begin{math}
	\ket{\Phi} = \alpha_1\ket{0} + \beta_1\ket{1} 
\end{math}

\begin{math}
	\ket{\Psi} = \begin{pmatrix}
	\alpha \\
	\beta
\end{pmatrix}
\end{math}

\begin{math}
\ket{\Psi} = \alpha\ket{0} \otimes \beta\ket{0} = \begin{pmatrix}
	a \\
	0
\end{pmatrix}
\otimes
\begin{pmatrix}
	b \\
	0
\end{pmatrix}
\end{math}

\begin{math}
\begin{pmatrix}
	a \\
	0
\end{pmatrix}
\otimes
\begin{pmatrix}
	b \\
	0
\end{pmatrix}
=
\begin{pmatrix}
	a \begin{pmatrix}
		b \\
		0
	\end{pmatrix} \\
	0 \begin{pmatrix}
		b \\
		0
	\end{pmatrix}
\end{pmatrix}
\end{math}

\begin{math}
\begin{pmatrix}
	a \begin{pmatrix}
		b \\
		0
	\end{pmatrix} \\
	0 \begin{pmatrix}
		b \\
		0
	\end{pmatrix}
\end{pmatrix}
=
\begin{pmatrix}
		ab \\
		0 \\
		0 \\
		0
\end{pmatrix}
\end{math}

\begin{math}
a\ket{0} \otimes b\ket{0} =
\begin{pmatrix}
		ab \\
		0 \\
		0 \\
		0
\end{pmatrix}
\end{math}

\end{document}
